Move some things

HeyVL.lean
@@ -1,1 +1,46 @@
 import HeyVL.Verify
+
+open Optimization.Notation
+open HeyLo
+
+abbrev NatLog.y : Ident := ⟨"y", .Nat⟩
+abbrev NatLog.c : Ident := ⟨"c", .Nat⟩
+
+open NatLog
+
+def NatLog := vc[𝒟, wp]
+  { ↑c + [0 < y] * ↑(y + nlog2(y)) }
+    while 0 < y inv(↑c + [0 < y] * ↑(y + nlog2(y))) {
+      { y := y / 2 } [1/2] { y := y - 1 } ; c := c + 1
+    }
+  { ↑c }
+
+theorem NatLog.soundess : NatLog.sound := by
+  apply NatLog.show_wp fun σ ↦ ?_
+  simp [NatLog]
+  simp [BinOp.sem, UnOp.sem, sem, Fun.sem]
+  set c : ℕ := σ c; set y : ℕ := σ y
+  intro c' y'
+  have : ∀ {a b : ENNReal}, (~~a ≤ b ↔ a = 0 ∨ b = ⊤) := by simp [compl]; grind [zero_le]
+  simp [this]; left
+  rcases y' with _ | y' <;> simp
+  grw [Nat.log2_div_2, (by gcongr; omega : Nat.log2 y' ≤ Nat.log2 (y' + 1))]
+  repeat rw [Nat.cast_add]
+  if h₁ : 0 < y' then
+    simp [h₁, (by omega : 0 < (y' + 1) / 2)]
+    grw [(by omega : (y' + 1) / 2 ≤ (y' + 1))]
+    simp [← ENNReal.toReal_le_toReal, ENNReal.mul_eq_top, ENNReal.toReal_add]
+    rw [ENNReal.toReal_sub_of_le]
+    · grind [ENNReal.toReal_natCast, ENNReal.toReal_one]
+    · simp; apply (Nat.le_log2 ?_).mpr <;> grind
+    · grind [ENNReal.natCast_ne_top]
+  else
+    have : y' = 0 := by omega
+    subst_eqs
+    ring_nf
+    grind [ENNReal.two_inv_mul_two, add_comm, CharP.cast_eq_zero, zero_add]
+
+/--
+info: 'NatLog.soundess' depends on axioms: [propext, Classical.choice, Lean.ofReduceBool, Lean.trustCompiler, Quot.sound]
+-/
+#guard_msgs in #print axioms NatLog.soundess
