PGCL.lean
@@ -10,19 +10,35 @@ import PGCL.IdleInduction
 ## Main definitions
 
 * `pGCL`: The definition of a variant of the _pGCL language_.
-* `pGCL.SmallStep`: The _small step operations semantics_ of pGCL.
-* `pGCL.𝒬`: The _induced operational Markov Decision Process_ (`MDP`) by the small step operational
-  semantics.
-* `pGCL.dwp`: The _weakest preexpectation transformer_ of a pGCL program.
-* `pGCL.op`: The _operational optimal expected cost transformer_ expressed as the optimal expected
-  cost of `pGCL.𝒬`.
-* `pGCL.dop_eq_dwp`: Theorem stating that the optimal expected cost is equal the weakest
-  preexpectation.
-* `pGCL.iSup_iInf_EC_eq_wp`: Theorem stating that the `⨅⨆` formulation of the optimal expected cost
-  is equal to the weakest preexpectation.
+* `pGCL.SmallStep`: The _small step operations semantics_ of pGCL. semantics.
+* `pGCL.wp`: The _weakest preexpectation transformer_ of a pGCL program.
+* `pGCL.wp_eq_op`: Theorem stating that the optimal expected cost is equal the weakest
+preexpectation.
+* `pGCL.iInf_iSup_EC_eq_wp`: Theorem stating that the `⨆⨅` formulation of the optimal expected cost
+is equal to the weakest preexpectation.
 -/
 
 open scoped Optimization.Notation
+
+theorem pGCL.iSup_iSup_EC_eq_wp [DecidableEq 𝒱] :
+      ⨆ 𝒮, ⨆ n, (𝕊 (𝒱:=𝒱) cost_t cost_p).mdp.EC ((𝕊 cost_t cost_p).cost X) 𝒮 n conf[@C,σ]
+    = wp[𝒜]⟦@C⟧ X σ := by
+  rw [wp_eq_op]
+  classical
+  have := congrFun ((𝕊 cost_t cost_p).mdp.iSup_iSup_EC_eq_lfp_Φ𝒜 (c:=(𝕊 _ _).cost X)) (.prog C σ)
+  simp at this
+  simp [this, iSup_comm]
+  rfl
+
+theorem pGCL.iInf_iSup_EC_eq_wp [DecidableEq 𝒱] :
+      ⨅ 𝒮, ⨆ n, (𝕊 (𝒱:=𝒱) cost_t cost_p).mdp.EC ((𝕊 cost_t cost_p).cost X) 𝒮 n conf[@C,σ]
+    = wp[𝒟]⟦@C⟧ X σ := by
+  rw [wp_eq_op]
+  classical
+  have := congrFun ((𝕊 cost_t cost_p).mdp.iInf_iSup_EC_eq_lfp_Φ𝒟 (c:=(𝕊 _ _).cost X)) (.prog C σ)
+  simp at this
+  simp [this]
+  rfl
 
 theorem pGCL.iSup_iSup_EC_eq_wfp [DecidableEq 𝒱] :
       ⨆ 𝒮, ⨆ n, (𝕊 (𝒱:=𝒱) cost_t' cost_p').mdp.EC ((𝕊 cost_t' cost_p').cost X) 𝒮 n conf[@C,σ]
@@ -44,6 +60,10 @@ theorem pGCL.iInf_iSup_EC_eq_wfp [DecidableEq 𝒱] :
   rw [← MDP.iSup_iInf_EC_eq_lfp_Φ𝒟, MDP.iSup_iInf_EC_eq_iInf_iSup_EC]
   simp only [iInf_apply, iSup_apply]
 
+/-- info: 'pGCL.iSup_iSup_EC_eq_wp' depends on axioms: [propext, Classical.choice, Quot.sound] -/
+#guard_msgs in #print axioms pGCL.iSup_iSup_EC_eq_wp
+/-- info: 'pGCL.iInf_iSup_EC_eq_wp' depends on axioms: [propext, Classical.choice, Quot.sound] -/
+#guard_msgs in #print axioms pGCL.iInf_iSup_EC_eq_wp
 /-- info: 'pGCL.iSup_iSup_EC_eq_wfp' depends on axioms: [propext, Classical.choice, Quot.sound] -/
 #guard_msgs in #print axioms pGCL.iSup_iSup_EC_eq_wfp
 /-- info: 'pGCL.iInf_iSup_EC_eq_wfp' depends on axioms: [propext, Classical.choice, Quot.sound] -/
